theories/CertiGC/model/constants.v
@@ -20,12 +20,12 @@ Definition SPACE_STRUCT_SIZE: Z
 
 Definition MAX_SPACES: Z := 12.
 Definition MAX_SPACES_eq: MAX_SPACES = 12 := eq_refl.
-Hint Rewrite MAX_SPACES_eq: rep_lia.
+#[global]Hint Rewrite MAX_SPACES_eq: rep_lia.
 Global Opaque MAX_SPACES.
 
 Definition NURSERY_SIZE: Z := Z.shiftl 1 16.
 Definition NURSERY_SIZE_eq: NURSERY_SIZE = Z.shiftl 1 16 := eq_refl.
-Hint Rewrite NURSERY_SIZE_eq: rep_lia.
+#[global]Hint Rewrite NURSERY_SIZE_eq: rep_lia.
 Global Opaque NURSERY_SIZE.
 
 Definition generation_size (n: nat) := (NURSERY_SIZE * two_p (Z.of_nat n))%Z.
@@ -51,12 +51,12 @@ Qed.
 
 Definition MAX_ARGS: Z := 1024.
 Definition MAX_ARGS_eq: MAX_ARGS = 1024 := eq_refl.
-Hint Rewrite MAX_ARGS_eq: rep_lia.
+#[global]Hint Rewrite MAX_ARGS_eq: rep_lia.
 Global Opaque MAX_ARGS.
 
 Definition NO_SCAN_TAG: Z := 251.
 Definition NO_SCAN_TAG_eq: NO_SCAN_TAG = 251 := eq_refl.
-Hint Rewrite NO_SCAN_TAG_eq: rep_lia.
+#[global]Hint Rewrite NO_SCAN_TAG_eq: rep_lia.
 Global Opaque NO_SCAN_TAG.
 
 
