theories/CertiGC/vst/ast/env_graph_gc.v
@@ -2,10 +2,8 @@ From VST Require Export floyd.proofauto.
 From VST Require Export floyd.library.
 From CertiGC Require Export CertiGC.vst.clightgen.gc.
 
-Instance CompSpecs : compspecs. make_compspecs prog. Defined.
+#[global]Instance CompSpecs : compspecs. make_compspecs prog. Defined.
 Definition Vprog : varspecs. mk_varspecs prog. Defined.
-
-Definition tvalue: type := tptr tvoid.
 
 Definition thread_info_type : type := Tstruct _thread_info noattr.
 Definition space_type : type := Tstruct _space noattr.
