theories/CertiGC/vst/clightgen/x86_32-linux/gc.v
@@ -508,67 +508,69 @@ Definition v_stderr := {|
 Definition f_test_int_or_ptr := {|
   fn_return := tint;
   fn_callconv := cc_default;
-  fn_params := ((_x, (tptr tvoid)) :: nil);
+  fn_params := ((_x, (talignas 2%N (tptr tvoid))) :: nil);
   fn_vars := nil;
   fn_temps := nil;
   fn_body :=
 (Sreturn (Some (Ecast
-                 (Ebinop Oand (Ecast (Etempvar _x (tptr tvoid)) tint)
+                 (Ebinop Oand
+                   (Ecast (Etempvar _x (talignas 2%N (tptr tvoid))) tint)
                    (Econst_int (Int.repr 1) tint) tint) tint)))
 |}.
 
 Definition f_int_or_ptr_to_int := {|
   fn_return := tint;
   fn_callconv := cc_default;
-  fn_params := ((_x, (tptr tvoid)) :: nil);
+  fn_params := ((_x, (talignas 2%N (tptr tvoid))) :: nil);
   fn_vars := nil;
   fn_temps := nil;
   fn_body :=
-(Sreturn (Some (Ecast (Etempvar _x (tptr tvoid)) tint)))
+(Sreturn (Some (Ecast (Etempvar _x (talignas 2%N (tptr tvoid))) tint)))
 |}.
 
 Definition f_int_or_ptr_to_ptr := {|
   fn_return := (tptr tvoid);
   fn_callconv := cc_default;
-  fn_params := ((_x, (tptr tvoid)) :: nil);
+  fn_params := ((_x, (talignas 2%N (tptr tvoid))) :: nil);
   fn_vars := nil;
   fn_temps := nil;
   fn_body :=
-(Sreturn (Some (Ecast (Etempvar _x (tptr tvoid)) (tptr tvoid))))
+(Sreturn (Some (Ecast (Etempvar _x (talignas 2%N (tptr tvoid))) (tptr tvoid))))
 |}.
 
 Definition f_int_to_int_or_ptr := {|
-  fn_return := (tptr tvoid);
+  fn_return := (talignas 2%N (tptr tvoid));
   fn_callconv := cc_default;
   fn_params := ((_x, tint) :: nil);
   fn_vars := nil;
   fn_temps := nil;
   fn_body :=
-(Sreturn (Some (Ecast (Etempvar _x tint) (tptr tvoid))))
+(Sreturn (Some (Ecast (Etempvar _x tint) (talignas 2%N (tptr tvoid)))))
 |}.
 
 Definition f_ptr_to_int_or_ptr := {|
-  fn_return := (tptr tvoid);
+  fn_return := (talignas 2%N (tptr tvoid));
   fn_callconv := cc_default;
   fn_params := ((_x, (tptr tvoid)) :: nil);
   fn_vars := nil;
   fn_temps := nil;
   fn_body :=
-(Sreturn (Some (Ecast (Etempvar _x (tptr tvoid)) (tptr tvoid))))
+(Sreturn (Some (Ecast (Etempvar _x (tptr tvoid)) (talignas 2%N (tptr tvoid)))))
 |}.
 
 Definition f_Is_block := {|
   fn_return := tint;
   fn_callconv := cc_default;
-  fn_params := ((_x, (tptr tvoid)) :: nil);
+  fn_params := ((_x, (talignas 2%N (tptr tvoid))) :: nil);
   fn_vars := nil;
   fn_temps := ((_t'1, tint) :: nil);
   fn_body :=
 (Ssequence
   (Scall (Some _t'1)
-    (Evar _test_int_or_ptr (Tfunction (Tcons (tptr tvoid) Tnil) tint
+    (Evar _test_int_or_ptr (Tfunction
+                             (Tcons (talignas 2%N (tptr tvoid)) Tnil) tint
                              cc_default))
-    ((Etempvar _x (tptr tvoid)) :: nil))
+    ((Etempvar _x (talignas 2%N (tptr tvoid))) :: nil))
   (Sreturn (Some (Ebinop Oeq (Etempvar _t'1 tint)
                    (Econst_int (Int.repr 0) tint) tint))))
 |}.
@@ -604,19 +606,21 @@ Definition f_abort_with := {|
 Definition f_Is_from := {|
   fn_return := tint;
   fn_callconv := cc_default;
-  fn_params := ((_from_start, (tptr (tptr tvoid))) ::
-                (_from_limit, (tptr (tptr tvoid))) ::
-                (_v, (tptr (tptr tvoid))) :: nil);
+  fn_params := ((_from_start, (tptr (talignas 2%N (tptr tvoid)))) ::
+                (_from_limit, (tptr (talignas 2%N (tptr tvoid)))) ::
+                (_v, (tptr (talignas 2%N (tptr tvoid)))) :: nil);
   fn_vars := nil;
   fn_temps := ((_t'1, tint) :: nil);
   fn_body :=
 (Ssequence
-  (Sifthenelse (Ebinop Ole (Etempvar _from_start (tptr (tptr tvoid)))
-                 (Etempvar _v (tptr (tptr tvoid))) tint)
+  (Sifthenelse (Ebinop Ole
+                 (Etempvar _from_start (tptr (talignas 2%N (tptr tvoid))))
+                 (Etempvar _v (tptr (talignas 2%N (tptr tvoid)))) tint)
     (Sset _t'1
       (Ecast
-        (Ebinop Olt (Etempvar _v (tptr (tptr tvoid)))
-          (Etempvar _from_limit (tptr (tptr tvoid))) tint) tbool))
+        (Ebinop Olt (Etempvar _v (tptr (talignas 2%N (tptr tvoid))))
+          (Etempvar _from_limit (tptr (talignas 2%N (tptr tvoid)))) tint)
+        tbool))
     (Sset _t'1 (Econst_int (Int.repr 0) tint)))
   (Sreturn (Some (Etempvar _t'1 tint))))
 |}.
@@ -624,48 +628,59 @@ Definition f_Is_from := {|
 Definition f_forward := {|
   fn_return := tvoid;
   fn_callconv := cc_default;
-  fn_params := ((_from_start, (tptr (tptr tvoid))) ::
-                (_from_limit, (tptr (tptr tvoid))) ::
-                (_next, (tptr (tptr (tptr tvoid)))) ::
-                (_p, (tptr (tptr tvoid))) :: (_depth, tint) :: nil);
+  fn_params := ((_from_start, (tptr (talignas 2%N (tptr tvoid)))) ::
+                (_from_limit, (tptr (talignas 2%N (tptr tvoid)))) ::
+                (_next, (tptr (tptr (talignas 2%N (tptr tvoid))))) ::
+                (_p, (tptr (talignas 2%N (tptr tvoid)))) :: (_depth, tint) ::
+                nil);
   fn_vars := nil;
-  fn_temps := ((_v, (tptr (tptr tvoid))) :: (_va, (tptr tvoid)) ::
-               (_hd, tuint) :: (_i, tint) :: (_sz, tint) ::
-               (_new, (tptr (tptr tvoid))) :: (_t'5, tint) :: (_t'4, tint) ::
-               (_t'3, (tptr tvoid)) :: (_t'2, (tptr tvoid)) ::
-               (_t'1, (tptr tvoid)) :: (_t'8, (tptr tvoid)) ::
-               (_t'7, (tptr (tptr tvoid))) :: (_t'6, (tptr tvoid)) :: nil);
+  fn_temps := ((_v, (tptr (talignas 2%N (tptr tvoid)))) ::
+               (_va, (talignas 2%N (tptr tvoid))) :: (_hd, tuint) ::
+               (_i, tint) :: (_sz, tint) ::
+               (_new, (tptr (talignas 2%N (tptr tvoid)))) :: (_t'5, tint) ::
+               (_t'4, tint) :: (_t'3, (talignas 2%N (tptr tvoid))) ::
+               (_t'2, (talignas 2%N (tptr tvoid))) :: (_t'1, (tptr tvoid)) ::
+               (_t'8, (talignas 2%N (tptr tvoid))) ::
+               (_t'7, (tptr (talignas 2%N (tptr tvoid)))) ::
+               (_t'6, (talignas 2%N (tptr tvoid))) :: nil);
   fn_body :=
 (Ssequence
-  (Sset _va (Ederef (Etempvar _p (tptr (tptr tvoid))) (tptr tvoid)))
+  (Sset _va
+    (Ederef (Etempvar _p (tptr (talignas 2%N (tptr tvoid))))
+      (talignas 2%N (tptr tvoid))))
   (Ssequence
     (Scall (Some _t'5)
-      (Evar _Is_block (Tfunction (Tcons (tptr tvoid) Tnil) tint cc_default))
-      ((Etempvar _va (tptr tvoid)) :: nil))
+      (Evar _Is_block (Tfunction (Tcons (talignas 2%N (tptr tvoid)) Tnil)
+                        tint cc_default))
+      ((Etempvar _va (talignas 2%N (tptr tvoid))) :: nil))
     (Sifthenelse (Etempvar _t'5 tint)
       (Ssequence
         (Ssequence
           (Scall (Some _t'1)
-            (Evar _int_or_ptr_to_ptr (Tfunction (Tcons (tptr tvoid) Tnil)
-                                       (tptr tvoid) cc_default))
-            ((Etempvar _va (tptr tvoid)) :: nil))
-          (Sset _v (Ecast (Etempvar _t'1 (tptr tvoid)) (tptr (tptr tvoid)))))
+            (Evar _int_or_ptr_to_ptr (Tfunction
+                                       (Tcons (talignas 2%N (tptr tvoid))
+                                         Tnil) (tptr tvoid) cc_default))
+            ((Etempvar _va (talignas 2%N (tptr tvoid))) :: nil))
+          (Sset _v
+            (Ecast (Etempvar _t'1 (tptr tvoid))
+              (tptr (talignas 2%N (tptr tvoid))))))
         (Ssequence
           (Scall (Some _t'4)
             (Evar _Is_from (Tfunction
-                             (Tcons (tptr (tptr tvoid))
-                               (Tcons (tptr (tptr tvoid))
-                                 (Tcons (tptr (tptr tvoid)) Tnil))) tint
-                             cc_default))
-            ((Etempvar _from_start (tptr (tptr tvoid))) ::
-             (Etempvar _from_limit (tptr (tptr tvoid))) ::
-             (Etempvar _v (tptr (tptr tvoid))) :: nil))
+                             (Tcons (tptr (talignas 2%N (tptr tvoid)))
+                               (Tcons (tptr (talignas 2%N (tptr tvoid)))
+                                 (Tcons (tptr (talignas 2%N (tptr tvoid)))
+                                   Tnil))) tint cc_default))
+            ((Etempvar _from_start (tptr (talignas 2%N (tptr tvoid)))) ::
+             (Etempvar _from_limit (tptr (talignas 2%N (tptr tvoid)))) ::
+             (Etempvar _v (tptr (talignas 2%N (tptr tvoid)))) :: nil))
           (Sifthenelse (Etempvar _t'4 tint)
             (Ssequence
               (Sset _hd
                 (Ederef
                   (Ebinop Oadd
-                    (Ecast (Etempvar _v (tptr (tptr tvoid))) (tptr tuint))
+                    (Ecast (Etempvar _v (tptr (talignas 2%N (tptr tvoid))))
+                      (tptr tuint))
                     (Eunop Oneg (Econst_int (Int.repr 1) tint) tint)
                     (tptr tuint)) tuint))
               (Sifthenelse (Ebinop Oeq (Etempvar _hd tuint)
@@ -674,12 +689,16 @@ Definition f_forward := {|
                   (Sset _t'8
                     (Ederef
                       (Ebinop Oadd
-                        (Ecast (Etempvar _v (tptr (tptr tvoid)))
-                          (tptr (tptr tvoid))) (Econst_int (Int.repr 0) tint)
-                        (tptr (tptr tvoid))) (tptr tvoid)))
+                        (Ecast
+                          (Etempvar _v (tptr (talignas 2%N (tptr tvoid))))
+                          (tptr (talignas 2%N (tptr tvoid))))
+                        (Econst_int (Int.repr 0) tint)
+                        (tptr (talignas 2%N (tptr tvoid))))
+                      (talignas 2%N (tptr tvoid))))
                   (Sassign
-                    (Ederef (Etempvar _p (tptr (tptr tvoid))) (tptr tvoid))
-                    (Etempvar _t'8 (tptr tvoid))))
+                    (Ederef (Etempvar _p (tptr (talignas 2%N (tptr tvoid))))
+                      (talignas 2%N (tptr tvoid)))
+                    (Etempvar _t'8 (talignas 2%N (tptr tvoid)))))
                 (Ssequence
                   (Sset _sz
                     (Ecast
@@ -688,22 +707,29 @@ Definition f_forward := {|
                   (Ssequence
                     (Ssequence
                       (Sset _t'7
-                        (Ederef (Etempvar _next (tptr (tptr (tptr tvoid))))
-                          (tptr (tptr tvoid))))
+                        (Ederef
+                          (Etempvar _next (tptr (tptr (talignas 2%N (tptr tvoid)))))
+                          (tptr (talignas 2%N (tptr tvoid)))))
                       (Sset _new
-                        (Ebinop Oadd (Etempvar _t'7 (tptr (tptr tvoid)))
-                          (Econst_int (Int.repr 1) tint) (tptr (tptr tvoid)))))
+                        (Ebinop Oadd
+                          (Etempvar _t'7 (tptr (talignas 2%N (tptr tvoid))))
+                          (Econst_int (Int.repr 1) tint)
+                          (tptr (talignas 2%N (tptr tvoid))))))
                     (Ssequence
                       (Sassign
-                        (Ederef (Etempvar _next (tptr (tptr (tptr tvoid))))
-                          (tptr (tptr tvoid)))
-                        (Ebinop Oadd (Etempvar _new (tptr (tptr tvoid)))
-                          (Etempvar _sz tint) (tptr (tptr tvoid))))
+                        (Ederef
+                          (Etempvar _next (tptr (tptr (talignas 2%N (tptr tvoid)))))
+                          (tptr (talignas 2%N (tptr tvoid))))
+                        (Ebinop Oadd
+                          (Etempvar _new (tptr (talignas 2%N (tptr tvoid))))
+                          (Etempvar _sz tint)
+                          (tptr (talignas 2%N (tptr tvoid)))))
                       (Ssequence
                         (Sassign
                           (Ederef
                             (Ebinop Oadd
-                              (Ecast (Etempvar _new (tptr (tptr tvoid)))
+                              (Ecast
+                                (Etempvar _new (tptr (talignas 2%N (tptr tvoid))))
                                 (tptr tuint))
                               (Eunop Oneg (Econst_int (Int.repr 1) tint)
                                 tint) (tptr tuint)) tuint)
@@ -722,19 +748,21 @@ Definition f_forward := {|
                                     (Ederef
                                       (Ebinop Oadd
                                         (Ecast
-                                          (Etempvar _v (tptr (tptr tvoid)))
-                                          (tptr (tptr tvoid)))
+                                          (Etempvar _v (tptr (talignas 2%N (tptr tvoid))))
+                                          (tptr (talignas 2%N (tptr tvoid))))
                                         (Etempvar _i tint)
-                                        (tptr (tptr tvoid))) (tptr tvoid)))
+                                        (tptr (talignas 2%N (tptr tvoid))))
+                                      (talignas 2%N (tptr tvoid))))
                                   (Sassign
                                     (Ederef
                                       (Ebinop Oadd
                                         (Ecast
-                                          (Etempvar _new (tptr (tptr tvoid)))
-                                          (tptr (tptr tvoid)))
+                                          (Etempvar _new (tptr (talignas 2%N (tptr tvoid))))
+                                          (tptr (talignas 2%N (tptr tvoid))))
                                         (Etempvar _i tint)
-                                        (tptr (tptr tvoid))) (tptr tvoid))
-                                    (Etempvar _t'6 (tptr tvoid)))))
+                                        (tptr (talignas 2%N (tptr tvoid))))
+                                      (talignas 2%N (tptr tvoid)))
+                                    (Etempvar _t'6 (talignas 2%N (tptr tvoid))))))
                               (Sset _i
                                 (Ebinop Oadd (Etempvar _i tint)
                                   (Econst_int (Int.repr 1) tint) tint))))
@@ -742,7 +770,8 @@ Definition f_forward := {|
                             (Sassign
                               (Ederef
                                 (Ebinop Oadd
-                                  (Ecast (Etempvar _v (tptr (tptr tvoid)))
+                                  (Ecast
+                                    (Etempvar _v (tptr (talignas 2%N (tptr tvoid))))
                                     (tptr tuint))
                                   (Eunop Oneg (Econst_int (Int.repr 1) tint)
                                     tint) (tptr tuint)) tuint)
@@ -754,19 +783,21 @@ Definition f_forward := {|
                                                              (Tcons
                                                                (tptr tvoid)
                                                                Tnil)
-                                                             (tptr tvoid)
+                                                             (talignas 2%N (tptr tvoid))
                                                              cc_default))
-                                  ((Ecast (Etempvar _new (tptr (tptr tvoid)))
+                                  ((Ecast
+                                     (Etempvar _new (tptr (talignas 2%N (tptr tvoid))))
                                      (tptr tvoid)) :: nil))
                                 (Sassign
                                   (Ederef
                                     (Ebinop Oadd
                                       (Ecast
-                                        (Etempvar _v (tptr (tptr tvoid)))
-                                        (tptr (tptr tvoid)))
+                                        (Etempvar _v (tptr (talignas 2%N (tptr tvoid))))
+                                        (tptr (talignas 2%N (tptr tvoid))))
                                       (Econst_int (Int.repr 0) tint)
-                                      (tptr (tptr tvoid))) (tptr tvoid))
-                                  (Etempvar _t'2 (tptr tvoid))))
+                                      (tptr (talignas 2%N (tptr tvoid))))
+                                    (talignas 2%N (tptr tvoid)))
+                                  (Etempvar _t'2 (talignas 2%N (tptr tvoid)))))
                               (Ssequence
                                 (Ssequence
                                   (Scall (Some _t'3)
@@ -774,15 +805,16 @@ Definition f_forward := {|
                                                                (Tcons
                                                                  (tptr tvoid)
                                                                  Tnil)
-                                                               (tptr tvoid)
+                                                               (talignas 2%N (tptr tvoid))
                                                                cc_default))
                                     ((Ecast
-                                       (Etempvar _new (tptr (tptr tvoid)))
+                                       (Etempvar _new (tptr (talignas 2%N (tptr tvoid))))
                                        (tptr tvoid)) :: nil))
                                   (Sassign
-                                    (Ederef (Etempvar _p (tptr (tptr tvoid)))
-                                      (tptr tvoid))
-                                    (Etempvar _t'3 (tptr tvoid))))
+                                    (Ederef
+                                      (Etempvar _p (tptr (talignas 2%N (tptr tvoid))))
+                                      (talignas 2%N (tptr tvoid)))
+                                    (Etempvar _t'3 (talignas 2%N (tptr tvoid)))))
                                 (Sifthenelse (Ebinop Ogt
                                                (Etempvar _depth tint)
                                                (Econst_int (Int.repr 0) tint)
@@ -800,26 +832,26 @@ Definition f_forward := {|
                                         (Scall None
                                           (Evar _forward (Tfunction
                                                            (Tcons
-                                                             (tptr (tptr tvoid))
+                                                             (tptr (talignas 2%N (tptr tvoid)))
                                                              (Tcons
-                                                               (tptr (tptr tvoid))
+                                                               (tptr (talignas 2%N (tptr tvoid)))
                                                                (Tcons
-                                                                 (tptr (tptr (tptr tvoid)))
+                                                                 (tptr (tptr (talignas 2%N (tptr tvoid))))
                                                                  (Tcons
-                                                                   (tptr (tptr tvoid))
+                                                                   (tptr (talignas 2%N (tptr tvoid)))
                                                                    (Tcons
                                                                     tint
                                                                     Tnil)))))
                                                            tvoid cc_default))
-                                          ((Etempvar _from_start (tptr (tptr tvoid))) ::
-                                           (Etempvar _from_limit (tptr (tptr tvoid))) ::
-                                           (Etempvar _next (tptr (tptr (tptr tvoid)))) ::
+                                          ((Etempvar _from_start (tptr (talignas 2%N (tptr tvoid)))) ::
+                                           (Etempvar _from_limit (tptr (talignas 2%N (tptr tvoid)))) ::
+                                           (Etempvar _next (tptr (tptr (talignas 2%N (tptr tvoid))))) ::
                                            (Ebinop Oadd
                                              (Ecast
-                                               (Etempvar _new (tptr (tptr tvoid)))
-                                               (tptr (tptr tvoid)))
+                                               (Etempvar _new (tptr (talignas 2%N (tptr tvoid))))
+                                               (tptr (talignas 2%N (tptr tvoid))))
                                              (Etempvar _i tint)
-                                             (tptr (tptr tvoid))) ::
+                                             (tptr (talignas 2%N (tptr tvoid)))) ::
                                            (Ebinop Osub
                                              (Etempvar _depth tint)
                                              (Econst_int (Int.repr 1) tint)
@@ -849,14 +881,15 @@ Definition v___func__ := {|
 Definition f_forward_roots := {|
   fn_return := tvoid;
   fn_callconv := cc_default;
-  fn_params := ((_from_start, (tptr (tptr tvoid))) ::
-                (_from_limit, (tptr (tptr tvoid))) ::
-                (_next, (tptr (tptr (tptr tvoid)))) :: (_fi, (tptr tuint)) ::
+  fn_params := ((_from_start, (tptr (talignas 2%N (tptr tvoid)))) ::
+                (_from_limit, (tptr (talignas 2%N (tptr tvoid)))) ::
+                (_next, (tptr (tptr (talignas 2%N (tptr tvoid))))) ::
+                (_fi, (tptr tuint)) ::
                 (_ti, (tptr (Tstruct _thread_info noattr))) :: nil);
   fn_vars := nil;
-  fn_temps := ((_args, (tptr (tptr tvoid))) :: (_n, tuint) :: (_i, tuint) ::
-               (_roots, (tptr tuint)) :: (_t'2, tuint) :: (_t'1, tuint) ::
-               nil);
+  fn_temps := ((_args, (tptr (talignas 2%N (tptr tvoid)))) :: (_n, tuint) ::
+               (_i, tuint) :: (_roots, (tptr tuint)) :: (_t'2, tuint) ::
+               (_t'1, tuint) :: nil);
   fn_body :=
 (Ssequence
   (Sset _roots
@@ -871,7 +904,8 @@ Definition f_forward_roots := {|
       (Sset _args
         (Efield
           (Ederef (Etempvar _ti (tptr (Tstruct _thread_info noattr)))
-            (Tstruct _thread_info noattr)) _args (tarray (tptr tvoid) 1024)))
+            (Tstruct _thread_info noattr)) _args
+          (tarray (talignas 2%N (tptr tvoid)) 1024)))
       (Ssequence
         (Sset _i (Econst_int (Int.repr 0) tint))
         (Sloop
@@ -907,17 +941,22 @@ Definition f_forward_roots := {|
                       (Etempvar _i tuint) (tptr tuint)) tuint))
                 (Scall None
                   (Evar _forward (Tfunction
-                                   (Tcons (tptr (tptr tvoid))
-                                     (Tcons (tptr (tptr tvoid))
-                                       (Tcons (tptr (tptr (tptr tvoid)))
-                                         (Tcons (tptr (tptr tvoid))
+                                   (Tcons (tptr (talignas 2%N (tptr tvoid)))
+                                     (Tcons
+                                       (tptr (talignas 2%N (tptr tvoid)))
+                                       (Tcons
+                                         (tptr (tptr (talignas 2%N (tptr tvoid))))
+                                         (Tcons
+                                           (tptr (talignas 2%N (tptr tvoid)))
                                            (Tcons tint Tnil))))) tvoid
                                    cc_default))
-                  ((Etempvar _from_start (tptr (tptr tvoid))) ::
-                   (Etempvar _from_limit (tptr (tptr tvoid))) ::
-                   (Etempvar _next (tptr (tptr (tptr tvoid)))) ::
-                   (Ebinop Oadd (Etempvar _args (tptr (tptr tvoid)))
-                     (Etempvar _t'1 tuint) (tptr (tptr tvoid))) ::
+                  ((Etempvar _from_start (tptr (talignas 2%N (tptr tvoid)))) ::
+                   (Etempvar _from_limit (tptr (talignas 2%N (tptr tvoid)))) ::
+                   (Etempvar _next (tptr (tptr (talignas 2%N (tptr tvoid))))) ::
+                   (Ebinop Oadd
+                     (Etempvar _args (tptr (talignas 2%N (tptr tvoid))))
+                     (Etempvar _t'1 tuint)
+                     (tptr (talignas 2%N (tptr tvoid)))) ::
                    (Econst_int (Int.repr 0) tint) :: nil)))))
           (Sset _i
             (Ebinop Oadd (Etempvar _i tuint) (Econst_int (Int.repr 1) tint)
@@ -927,31 +966,34 @@ Definition f_forward_roots := {|
 Definition f_do_scan := {|
   fn_return := tvoid;
   fn_callconv := cc_default;
-  fn_params := ((_from_start, (tptr (tptr tvoid))) ::
-                (_from_limit, (tptr (tptr tvoid))) ::
-                (_scan, (tptr (tptr tvoid))) ::
-                (_next, (tptr (tptr (tptr tvoid)))) :: nil);
+  fn_params := ((_from_start, (tptr (talignas 2%N (tptr tvoid)))) ::
+                (_from_limit, (tptr (talignas 2%N (tptr tvoid)))) ::
+                (_scan, (tptr (talignas 2%N (tptr tvoid)))) ::
+                (_next, (tptr (tptr (talignas 2%N (tptr tvoid))))) :: nil);
   fn_vars := nil;
-  fn_temps := ((_s, (tptr (tptr tvoid))) :: (_hd, tuint) :: (_sz, tuint) ::
-               (_tag, tint) :: (_j, tint) :: (_t'1, (tptr (tptr tvoid))) ::
-               nil);
+  fn_temps := ((_s, (tptr (talignas 2%N (tptr tvoid)))) :: (_hd, tuint) ::
+               (_sz, tuint) :: (_tag, tint) :: (_j, tint) ::
+               (_t'1, (tptr (talignas 2%N (tptr tvoid)))) :: nil);
   fn_body :=
 (Ssequence
-  (Sset _s (Etempvar _scan (tptr (tptr tvoid))))
+  (Sset _s (Etempvar _scan (tptr (talignas 2%N (tptr tvoid)))))
   (Sloop
     (Ssequence
       (Ssequence
         (Sset _t'1
-          (Ederef (Etempvar _next (tptr (tptr (tptr tvoid))))
-            (tptr (tptr tvoid))))
-        (Sifthenelse (Ebinop Olt (Etempvar _s (tptr (tptr tvoid)))
-                       (Etempvar _t'1 (tptr (tptr tvoid))) tint)
+          (Ederef (Etempvar _next (tptr (tptr (talignas 2%N (tptr tvoid)))))
+            (tptr (talignas 2%N (tptr tvoid)))))
+        (Sifthenelse (Ebinop Olt
+                       (Etempvar _s (tptr (talignas 2%N (tptr tvoid))))
+                       (Etempvar _t'1 (tptr (talignas 2%N (tptr tvoid))))
+                       tint)
           Sskip
           Sbreak))
       (Ssequence
         (Sset _hd
-          (Ederef (Ecast (Etempvar _s (tptr (tptr tvoid))) (tptr tuint))
-            tuint))
+          (Ederef
+            (Ecast (Etempvar _s (tptr (talignas 2%N (tptr tvoid))))
+              (tptr tuint)) tuint))
         (Ssequence
           (Sset _sz
             (Ecast
@@ -976,29 +1018,35 @@ Definition f_do_scan := {|
                         Sbreak)
                       (Scall None
                         (Evar _forward (Tfunction
-                                         (Tcons (tptr (tptr tvoid))
-                                           (Tcons (tptr (tptr tvoid))
+                                         (Tcons
+                                           (tptr (talignas 2%N (tptr tvoid)))
+                                           (Tcons
+                                             (tptr (talignas 2%N (tptr tvoid)))
                                              (Tcons
-                                               (tptr (tptr (tptr tvoid)))
-                                               (Tcons (tptr (tptr tvoid))
+                                               (tptr (tptr (talignas 2%N (tptr tvoid))))
+                                               (Tcons
+                                                 (tptr (talignas 2%N (tptr tvoid)))
                                                  (Tcons tint Tnil))))) tvoid
                                          cc_default))
-                        ((Etempvar _from_start (tptr (tptr tvoid))) ::
-                         (Etempvar _from_limit (tptr (tptr tvoid))) ::
-                         (Etempvar _next (tptr (tptr (tptr tvoid)))) ::
+                        ((Etempvar _from_start (tptr (talignas 2%N (tptr tvoid)))) ::
+                         (Etempvar _from_limit (tptr (talignas 2%N (tptr tvoid)))) ::
+                         (Etempvar _next (tptr (tptr (talignas 2%N (tptr tvoid))))) ::
                          (Ebinop Oadd
-                           (Ecast (Etempvar _s (tptr (tptr tvoid)))
-                             (tptr (tptr tvoid))) (Etempvar _j tint)
-                           (tptr (tptr tvoid))) ::
+                           (Ecast
+                             (Etempvar _s (tptr (talignas 2%N (tptr tvoid))))
+                             (tptr (talignas 2%N (tptr tvoid))))
+                           (Etempvar _j tint)
+                           (tptr (talignas 2%N (tptr tvoid)))) ::
                          (Econst_int (Int.repr 0) tint) :: nil)))
                     (Sset _j
                       (Ebinop Oadd (Etempvar _j tint)
                         (Econst_int (Int.repr 1) tint) tint))))
                 Sskip)
               (Sset _s
-                (Ebinop Oadd (Etempvar _s (tptr (tptr tvoid)))
+                (Ebinop Oadd (Etempvar _s (tptr (talignas 2%N (tptr tvoid))))
                   (Ebinop Oadd (Econst_int (Int.repr 1) tint)
-                    (Etempvar _sz tuint) tuint) (tptr (tptr tvoid)))))))))
+                    (Etempvar _sz tuint) tuint)
+                  (tptr (talignas 2%N (tptr tvoid))))))))))
     Sskip))
 |}.
 
@@ -1023,47 +1071,60 @@ Definition f_do_generation := {|
                 (_fi, (tptr tuint)) ::
                 (_ti, (tptr (Tstruct _thread_info noattr))) :: nil);
   fn_vars := nil;
-  fn_temps := ((_p, (tptr (tptr tvoid))) :: (_t'13, (tptr (tptr tvoid))) ::
-               (_t'12, (tptr (tptr tvoid))) ::
-               (_t'11, (tptr (tptr tvoid))) ::
-               (_t'10, (tptr (tptr tvoid))) :: (_t'9, (tptr (tptr tvoid))) ::
-               (_t'8, (tptr (tptr tvoid))) :: (_t'7, (tptr (tptr tvoid))) ::
-               (_t'6, (tptr (tptr tvoid))) :: (_t'5, (tptr (tptr tvoid))) ::
-               (_t'4, (tptr (tptr tvoid))) :: (_t'3, (tptr (tptr tvoid))) ::
+  fn_temps := ((_p, (tptr (talignas 2%N (tptr tvoid)))) ::
+               (_t'13, (tptr (talignas 2%N (tptr tvoid)))) ::
+               (_t'12, (tptr (talignas 2%N (tptr tvoid)))) ::
+               (_t'11, (tptr (talignas 2%N (tptr tvoid)))) ::
+               (_t'10, (tptr (talignas 2%N (tptr tvoid)))) ::
+               (_t'9, (tptr (talignas 2%N (tptr tvoid)))) ::
+               (_t'8, (tptr (talignas 2%N (tptr tvoid)))) ::
+               (_t'7, (tptr (talignas 2%N (tptr tvoid)))) ::
+               (_t'6, (tptr (talignas 2%N (tptr tvoid)))) ::
+               (_t'5, (tptr (talignas 2%N (tptr tvoid)))) ::
+               (_t'4, (tptr (talignas 2%N (tptr tvoid)))) ::
+               (_t'3, (tptr (talignas 2%N (tptr tvoid)))) ::
                (_t'2, (tptr (Tstruct __IO_FILE noattr))) ::
-               (_t'1, (tptr (tptr tvoid))) :: nil);
+               (_t'1, (tptr (talignas 2%N (tptr tvoid)))) :: nil);
   fn_body :=
 (Ssequence
   (Sset _p
     (Efield
       (Ederef (Etempvar _to (tptr (Tstruct _space noattr)))
-        (Tstruct _space noattr)) _next (tptr (tptr tvoid))))
+        (Tstruct _space noattr)) _next (tptr (talignas 2%N (tptr tvoid)))))
   (Ssequence
     (Ssequence
       (Sset _t'10
         (Efield
           (Ederef (Etempvar _from (tptr (Tstruct _space noattr)))
-            (Tstruct _space noattr)) _next (tptr (tptr tvoid))))
+            (Tstruct _space noattr)) _next
+          (tptr (talignas 2%N (tptr tvoid)))))
       (Ssequence
         (Sset _t'11
           (Efield
             (Ederef (Etempvar _from (tptr (Tstruct _space noattr)))
-              (Tstruct _space noattr)) _start (tptr (tptr tvoid))))
+              (Tstruct _space noattr)) _start
+            (tptr (talignas 2%N (tptr tvoid)))))
         (Ssequence
           (Sset _t'12
             (Efield
               (Ederef (Etempvar _to (tptr (Tstruct _space noattr)))
-                (Tstruct _space noattr)) _limit (tptr (tptr tvoid))))
+                (Tstruct _space noattr)) _limit
+              (tptr (talignas 2%N (tptr tvoid)))))
           (Ssequence
             (Sset _t'13
               (Efield
                 (Ederef (Etempvar _to (tptr (Tstruct _space noattr)))
-                  (Tstruct _space noattr)) _next (tptr (tptr tvoid))))
+                  (Tstruct _space noattr)) _next
+                (tptr (talignas 2%N (tptr tvoid)))))
             (Sifthenelse (Ebinop Ole
-                           (Ebinop Osub (Etempvar _t'10 (tptr (tptr tvoid)))
-                             (Etempvar _t'11 (tptr (tptr tvoid))) tint)
-                           (Ebinop Osub (Etempvar _t'12 (tptr (tptr tvoid)))
-                             (Etempvar _t'13 (tptr (tptr tvoid))) tint) tint)
+                           (Ebinop Osub
+                             (Etempvar _t'10 (tptr (talignas 2%N (tptr tvoid))))
+                             (Etempvar _t'11 (tptr (talignas 2%N (tptr tvoid))))
+                             tint)
+                           (Ebinop Osub
+                             (Etempvar _t'12 (tptr (talignas 2%N (tptr tvoid))))
+                             (Etempvar _t'13 (tptr (talignas 2%N (tptr tvoid))))
+                             tint) tint)
               Sskip
               (Scall None
                 (Evar ___assert_fail (Tfunction
@@ -1081,55 +1142,65 @@ Definition f_do_generation := {|
         (Sset _t'8
           (Efield
             (Ederef (Etempvar _from (tptr (Tstruct _space noattr)))
-              (Tstruct _space noattr)) _start (tptr (tptr tvoid))))
+              (Tstruct _space noattr)) _start
+            (tptr (talignas 2%N (tptr tvoid)))))
         (Ssequence
           (Sset _t'9
             (Efield
               (Ederef (Etempvar _from (tptr (Tstruct _space noattr)))
-                (Tstruct _space noattr)) _limit (tptr (tptr tvoid))))
+                (Tstruct _space noattr)) _limit
+              (tptr (talignas 2%N (tptr tvoid)))))
           (Scall None
             (Evar _forward_roots (Tfunction
-                                   (Tcons (tptr (tptr tvoid))
-                                     (Tcons (tptr (tptr tvoid))
-                                       (Tcons (tptr (tptr (tptr tvoid)))
+                                   (Tcons (tptr (talignas 2%N (tptr tvoid)))
+                                     (Tcons
+                                       (tptr (talignas 2%N (tptr tvoid)))
+                                       (Tcons
+                                         (tptr (tptr (talignas 2%N (tptr tvoid))))
                                          (Tcons (tptr tuint)
                                            (Tcons
                                              (tptr (Tstruct _thread_info noattr))
                                              Tnil))))) tvoid cc_default))
-            ((Etempvar _t'8 (tptr (tptr tvoid))) ::
-             (Etempvar _t'9 (tptr (tptr tvoid))) ::
+            ((Etempvar _t'8 (tptr (talignas 2%N (tptr tvoid)))) ::
+             (Etempvar _t'9 (tptr (talignas 2%N (tptr tvoid)))) ::
              (Eaddrof
                (Efield
                  (Ederef (Etempvar _to (tptr (Tstruct _space noattr)))
-                   (Tstruct _space noattr)) _next (tptr (tptr tvoid)))
-               (tptr (tptr (tptr tvoid)))) :: (Etempvar _fi (tptr tuint)) ::
+                   (Tstruct _space noattr)) _next
+                 (tptr (talignas 2%N (tptr tvoid))))
+               (tptr (tptr (talignas 2%N (tptr tvoid))))) ::
+             (Etempvar _fi (tptr tuint)) ::
              (Etempvar _ti (tptr (Tstruct _thread_info noattr))) :: nil))))
       (Ssequence
         (Ssequence
           (Sset _t'6
             (Efield
               (Ederef (Etempvar _from (tptr (Tstruct _space noattr)))
-                (Tstruct _space noattr)) _start (tptr (tptr tvoid))))
+                (Tstruct _space noattr)) _start
+              (tptr (talignas 2%N (tptr tvoid)))))
           (Ssequence
             (Sset _t'7
               (Efield
                 (Ederef (Etempvar _from (tptr (Tstruct _space noattr)))
-                  (Tstruct _space noattr)) _limit (tptr (tptr tvoid))))
+                  (Tstruct _space noattr)) _limit
+                (tptr (talignas 2%N (tptr tvoid)))))
             (Scall None
               (Evar _do_scan (Tfunction
-                               (Tcons (tptr (tptr tvoid))
-                                 (Tcons (tptr (tptr tvoid))
-                                   (Tcons (tptr (tptr tvoid))
-                                     (Tcons (tptr (tptr (tptr tvoid))) Tnil))))
-                               tvoid cc_default))
-              ((Etempvar _t'6 (tptr (tptr tvoid))) ::
-               (Etempvar _t'7 (tptr (tptr tvoid))) ::
-               (Etempvar _p (tptr (tptr tvoid))) ::
+                               (Tcons (tptr (talignas 2%N (tptr tvoid)))
+                                 (Tcons (tptr (talignas 2%N (tptr tvoid)))
+                                   (Tcons (tptr (talignas 2%N (tptr tvoid)))
+                                     (Tcons
+                                       (tptr (tptr (talignas 2%N (tptr tvoid))))
+                                       Tnil)))) tvoid cc_default))
+              ((Etempvar _t'6 (tptr (talignas 2%N (tptr tvoid)))) ::
+               (Etempvar _t'7 (tptr (talignas 2%N (tptr tvoid)))) ::
+               (Etempvar _p (tptr (talignas 2%N (tptr tvoid)))) ::
                (Eaddrof
                  (Efield
                    (Ederef (Etempvar _to (tptr (Tstruct _space noattr)))
-                     (Tstruct _space noattr)) _next (tptr (tptr tvoid)))
-                 (tptr (tptr (tptr tvoid)))) :: nil))))
+                     (Tstruct _space noattr)) _next
+                   (tptr (talignas 2%N (tptr tvoid))))
+                 (tptr (tptr (talignas 2%N (tptr tvoid))))) :: nil))))
         (Ssequence
           (Sifthenelse (Econst_int (Int.repr 0) tint)
             (Ssequence
@@ -1138,19 +1209,21 @@ Definition f_do_generation := {|
                 (Sset _t'3
                   (Efield
                     (Ederef (Etempvar _to (tptr (Tstruct _space noattr)))
-                      (Tstruct _space noattr)) _next (tptr (tptr tvoid))))
+                      (Tstruct _space noattr)) _next
+                    (tptr (talignas 2%N (tptr tvoid)))))
                 (Ssequence
                   (Sset _t'4
                     (Efield
                       (Ederef (Etempvar _from (tptr (Tstruct _space noattr)))
-                        (Tstruct _space noattr)) _next (tptr (tptr tvoid))))
+                        (Tstruct _space noattr)) _next
+                      (tptr (talignas 2%N (tptr tvoid)))))
                   (Ssequence
                     (Sset _t'5
                       (Efield
                         (Ederef
                           (Etempvar _from (tptr (Tstruct _space noattr)))
                           (Tstruct _space noattr)) _start
-                        (tptr (tptr tvoid))))
+                        (tptr (talignas 2%N (tptr tvoid)))))
                     (Scall None
                       (Evar _fprintf (Tfunction
                                        (Tcons
@@ -1160,23 +1233,28 @@ Definition f_do_generation := {|
                       ((Etempvar _t'2 (tptr (Tstruct __IO_FILE noattr))) ::
                        (Evar ___stringlit_4 (tarray tschar 19)) ::
                        (Ebinop Odiv
-                         (Ebinop Osub (Etempvar _t'3 (tptr (tptr tvoid)))
-                           (Etempvar _p (tptr (tptr tvoid))) tint)
+                         (Ebinop Osub
+                           (Etempvar _t'3 (tptr (talignas 2%N (tptr tvoid))))
+                           (Etempvar _p (tptr (talignas 2%N (tptr tvoid))))
+                           tint)
                          (Ecast
-                           (Ebinop Osub (Etempvar _t'4 (tptr (tptr tvoid)))
-                             (Etempvar _t'5 (tptr (tptr tvoid))) tint)
-                           tdouble) tdouble) :: nil))))))
+                           (Ebinop Osub
+                             (Etempvar _t'4 (tptr (talignas 2%N (tptr tvoid))))
+                             (Etempvar _t'5 (tptr (talignas 2%N (tptr tvoid))))
+                             tint) tdouble) tdouble) :: nil))))))
             Sskip)
           (Ssequence
             (Sset _t'1
               (Efield
                 (Ederef (Etempvar _from (tptr (Tstruct _space noattr)))
-                  (Tstruct _space noattr)) _start (tptr (tptr tvoid))))
+                  (Tstruct _space noattr)) _start
+                (tptr (talignas 2%N (tptr tvoid)))))
             (Sassign
               (Efield
                 (Ederef (Etempvar _from (tptr (Tstruct _space noattr)))
-                  (Tstruct _space noattr)) _next (tptr (tptr tvoid)))
-              (Etempvar _t'1 (tptr (tptr tvoid))))))))))
+                  (Tstruct _space noattr)) _next
+                (tptr (talignas 2%N (tptr tvoid))))
+              (Etempvar _t'1 (tptr (talignas 2%N (tptr tvoid)))))))))))
 |}.
 
 Definition f_create_space := {|
@@ -1184,8 +1262,8 @@ Definition f_create_space := {|
   fn_callconv := cc_default;
   fn_params := ((_s, (tptr (Tstruct _space noattr))) :: (_n, tuint) :: nil);
   fn_vars := nil;
-  fn_temps := ((_p, (tptr (tptr tvoid))) :: (_t'1, (tptr tvoid)) ::
-               (_t'2, tuint) :: nil);
+  fn_temps := ((_p, (tptr (talignas 2%N (tptr tvoid)))) ::
+               (_t'1, (tptr tvoid)) :: (_t'2, tuint) :: nil);
   fn_body :=
 (Ssequence
   (Ssequence
@@ -1200,11 +1278,14 @@ Definition f_create_space := {|
     (Ssequence
       (Scall (Some _t'1)
         (Evar _malloc (Tfunction (Tcons tuint Tnil) (tptr tvoid) cc_default))
-        ((Ebinop Omul (Etempvar _n tuint) (Esizeof (tptr tvoid) tuint) tuint) ::
-         nil))
-      (Sset _p (Ecast (Etempvar _t'1 (tptr tvoid)) (tptr (tptr tvoid)))))
+        ((Ebinop Omul (Etempvar _n tuint)
+           (Esizeof (talignas 2%N (tptr tvoid)) tuint) tuint) :: nil))
+      (Sset _p
+        (Ecast (Etempvar _t'1 (tptr tvoid))
+          (tptr (talignas 2%N (tptr tvoid))))))
     (Ssequence
-      (Sifthenelse (Ebinop Oeq (Etempvar _p (tptr (tptr tvoid)))
+      (Sifthenelse (Ebinop Oeq
+                     (Etempvar _p (tptr (talignas 2%N (tptr tvoid))))
                      (Ecast (Econst_int (Int.repr 0) tint) (tptr tvoid))
                      tint)
         (Scall None
@@ -1216,20 +1297,23 @@ Definition f_create_space := {|
         (Sassign
           (Efield
             (Ederef (Etempvar _s (tptr (Tstruct _space noattr)))
-              (Tstruct _space noattr)) _start (tptr (tptr tvoid)))
-          (Etempvar _p (tptr (tptr tvoid))))
+              (Tstruct _space noattr)) _start
+            (tptr (talignas 2%N (tptr tvoid))))
+          (Etempvar _p (tptr (talignas 2%N (tptr tvoid)))))
         (Ssequence
           (Sassign
             (Efield
               (Ederef (Etempvar _s (tptr (Tstruct _space noattr)))
-                (Tstruct _space noattr)) _next (tptr (tptr tvoid)))
-            (Etempvar _p (tptr (tptr tvoid))))
+                (Tstruct _space noattr)) _next
+              (tptr (talignas 2%N (tptr tvoid))))
+            (Etempvar _p (tptr (talignas 2%N (tptr tvoid)))))
           (Sassign
             (Efield
               (Ederef (Etempvar _s (tptr (Tstruct _space noattr)))
-                (Tstruct _space noattr)) _limit (tptr (tptr tvoid)))
-            (Ebinop Oadd (Etempvar _p (tptr (tptr tvoid)))
-              (Etempvar _n tuint) (tptr (tptr tvoid)))))))))
+                (Tstruct _space noattr)) _limit
+              (tptr (talignas 2%N (tptr tvoid))))
+            (Ebinop Oadd (Etempvar _p (tptr (talignas 2%N (tptr tvoid))))
+              (Etempvar _n tuint) (tptr (talignas 2%N (tptr tvoid))))))))))
 |}.
 
 Definition f_create_heap := {|
@@ -1287,7 +1371,8 @@ Definition f_create_heap := {|
                             (Tstruct _heap noattr)) _spaces
                           (tarray (Tstruct _space noattr) 12))
                         (Etempvar _i tint) (tptr (Tstruct _space noattr)))
-                      (Tstruct _space noattr)) _start (tptr (tptr tvoid)))
+                      (Tstruct _space noattr)) _start
+                    (tptr (talignas 2%N (tptr tvoid))))
                   (Ecast (Econst_int (Int.repr 0) tint) (tptr tvoid)))
                 (Ssequence
                   (Sassign
@@ -1300,7 +1385,8 @@ Definition f_create_heap := {|
                               (Tstruct _heap noattr)) _spaces
                             (tarray (Tstruct _space noattr) 12))
                           (Etempvar _i tint) (tptr (Tstruct _space noattr)))
-                        (Tstruct _space noattr)) _next (tptr (tptr tvoid)))
+                        (Tstruct _space noattr)) _next
+                      (tptr (talignas 2%N (tptr tvoid))))
                     (Ecast (Econst_int (Int.repr 0) tint) (tptr tvoid)))
                   (Sassign
                     (Efield
@@ -1312,7 +1398,8 @@ Definition f_create_heap := {|
                               (Tstruct _heap noattr)) _spaces
                             (tarray (Tstruct _space noattr) 12))
                           (Etempvar _i tint) (tptr (Tstruct _space noattr)))
-                        (Tstruct _space noattr)) _limit (tptr (tptr tvoid)))
+                        (Tstruct _space noattr)) _limit
+                      (tptr (talignas 2%N (tptr tvoid))))
                     (Ecast (Econst_int (Int.repr 0) tint) (tptr tvoid))))))
             (Sset _i
               (Ebinop Oadd (Etempvar _i tint) (Econst_int (Int.repr 1) tint)
@@ -1329,8 +1416,8 @@ Definition f_make_tinfo := {|
                (_tinfo, (tptr (Tstruct _thread_info noattr))) ::
                (_t'2, (tptr tvoid)) ::
                (_t'1, (tptr (Tstruct _heap noattr))) ::
-               (_t'4, (tptr (tptr tvoid))) :: (_t'3, (tptr (tptr tvoid))) ::
-               nil);
+               (_t'4, (tptr (talignas 2%N (tptr tvoid)))) ::
+               (_t'3, (tptr (talignas 2%N (tptr tvoid)))) :: nil);
   fn_body :=
 (Ssequence
   (Ssequence
@@ -1374,13 +1461,14 @@ Definition f_make_tinfo := {|
                       (tarray (Tstruct _space noattr) 12))
                     (Econst_int (Int.repr 0) tint)
                     (tptr (Tstruct _space noattr))) (Tstruct _space noattr))
-                _start (tptr (tptr tvoid))))
+                _start (tptr (talignas 2%N (tptr tvoid)))))
             (Sassign
               (Efield
                 (Ederef
                   (Etempvar _tinfo (tptr (Tstruct _thread_info noattr)))
-                  (Tstruct _thread_info noattr)) _alloc (tptr (tptr tvoid)))
-              (Etempvar _t'4 (tptr (tptr tvoid)))))
+                  (Tstruct _thread_info noattr)) _alloc
+                (tptr (talignas 2%N (tptr tvoid))))
+              (Etempvar _t'4 (tptr (talignas 2%N (tptr tvoid))))))
           (Ssequence
             (Ssequence
               (Sset _t'3
@@ -1393,13 +1481,15 @@ Definition f_make_tinfo := {|
                         (tarray (Tstruct _space noattr) 12))
                       (Econst_int (Int.repr 0) tint)
                       (tptr (Tstruct _space noattr)))
-                    (Tstruct _space noattr)) _limit (tptr (tptr tvoid))))
+                    (Tstruct _space noattr)) _limit
+                  (tptr (talignas 2%N (tptr tvoid)))))
               (Sassign
                 (Efield
                   (Ederef
                     (Etempvar _tinfo (tptr (Tstruct _thread_info noattr)))
                     (Tstruct _thread_info noattr)) _limit
-                  (tptr (tptr tvoid))) (Etempvar _t'3 (tptr (tptr tvoid)))))
+                  (tptr (talignas 2%N (tptr tvoid))))
+                (Etempvar _t'3 (tptr (talignas 2%N (tptr tvoid))))))
             (Sreturn (Some (Etempvar _tinfo (tptr (Tstruct _thread_info noattr)))))))))))
 |}.
 
@@ -1420,7 +1510,8 @@ Definition f_resume := {|
                 (_ti, (tptr (Tstruct _thread_info noattr))) :: nil);
   fn_vars := nil;
   fn_temps := ((_h, (tptr (Tstruct _heap noattr))) ::
-               (_lo, (tptr (tptr tvoid))) :: (_hi, (tptr (tptr tvoid))) ::
+               (_lo, (tptr (talignas 2%N (tptr tvoid)))) ::
+               (_hi, (tptr (talignas 2%N (tptr tvoid)))) ::
                (_num_allocs, tuint) :: nil);
   fn_body :=
 (Ssequence
@@ -1457,7 +1548,7 @@ Definition f_resume := {|
                   (tarray (Tstruct _space noattr) 12))
                 (Econst_int (Int.repr 0) tint)
                 (tptr (Tstruct _space noattr))) (Tstruct _space noattr))
-            _start (tptr (tptr tvoid))))
+            _start (tptr (talignas 2%N (tptr tvoid)))))
         (Ssequence
           (Sset _hi
             (Efield
@@ -1469,12 +1560,13 @@ Definition f_resume := {|
                     (tarray (Tstruct _space noattr) 12))
                   (Econst_int (Int.repr 0) tint)
                   (tptr (Tstruct _space noattr))) (Tstruct _space noattr))
-              _limit (tptr (tptr tvoid))))
+              _limit (tptr (talignas 2%N (tptr tvoid)))))
           (Ssequence
             (Sifthenelse (Ebinop Olt
-                           (Ebinop Osub (Etempvar _hi (tptr (tptr tvoid)))
-                             (Etempvar _lo (tptr (tptr tvoid))) tint)
-                           (Etempvar _num_allocs tuint) tint)
+                           (Ebinop Osub
+                             (Etempvar _hi (tptr (talignas 2%N (tptr tvoid))))
+                             (Etempvar _lo (tptr (talignas 2%N (tptr tvoid))))
+                             tint) (Etempvar _num_allocs tuint) tint)
               (Scall None
                 (Evar _abort_with (Tfunction (Tcons (tptr tschar) Tnil) tvoid
                                     cc_default))
@@ -1485,12 +1577,14 @@ Definition f_resume := {|
                 (Efield
                   (Ederef (Etempvar _ti (tptr (Tstruct _thread_info noattr)))
                     (Tstruct _thread_info noattr)) _alloc
-                  (tptr (tptr tvoid))) (Etempvar _lo (tptr (tptr tvoid))))
+                  (tptr (talignas 2%N (tptr tvoid))))
+                (Etempvar _lo (tptr (talignas 2%N (tptr tvoid)))))
               (Sassign
                 (Efield
                   (Ederef (Etempvar _ti (tptr (Tstruct _thread_info noattr)))
                     (Tstruct _thread_info noattr)) _limit
-                  (tptr (tptr tvoid))) (Etempvar _hi (tptr (tptr tvoid)))))))))))
+                  (tptr (talignas 2%N (tptr tvoid))))
+                (Etempvar _hi (tptr (talignas 2%N (tptr tvoid))))))))))))
 |}.
 
 Definition v___func____3 := {|
@@ -1514,13 +1608,15 @@ Definition f_garbage_collect := {|
                 (_ti, (tptr (Tstruct _thread_info noattr))) :: nil);
   fn_vars := nil;
   fn_temps := ((_h, (tptr (Tstruct _heap noattr))) :: (_i, tint) ::
-               (_w, tint) :: (_t'9, (tptr (tptr tvoid))) ::
-               (_t'8, (tptr (tptr tvoid))) :: (_t'7, (tptr (tptr tvoid))) ::
-               (_t'6, (tptr (tptr tvoid))) ::
+               (_w, tint) :: (_t'9, (tptr (talignas 2%N (tptr tvoid)))) ::
+               (_t'8, (tptr (talignas 2%N (tptr tvoid)))) ::
+               (_t'7, (tptr (talignas 2%N (tptr tvoid)))) ::
+               (_t'6, (tptr (talignas 2%N (tptr tvoid)))) ::
                (_t'5, (tptr (Tstruct __IO_FILE noattr))) ::
-               (_t'4, (tptr (tptr tvoid))) :: (_t'3, (tptr (tptr tvoid))) ::
-               (_t'2, (tptr (tptr tvoid))) :: (_t'1, (tptr (tptr tvoid))) ::
-               nil);
+               (_t'4, (tptr (talignas 2%N (tptr tvoid)))) ::
+               (_t'3, (tptr (talignas 2%N (tptr tvoid)))) ::
+               (_t'2, (tptr (talignas 2%N (tptr tvoid)))) ::
+               (_t'1, (tptr (talignas 2%N (tptr tvoid)))) :: nil);
   fn_body :=
 (Ssequence
   (Sset _h
@@ -1532,7 +1628,8 @@ Definition f_garbage_collect := {|
       (Sset _t'9
         (Efield
           (Ederef (Etempvar _ti (tptr (Tstruct _thread_info noattr)))
-            (Tstruct _thread_info noattr)) _alloc (tptr (tptr tvoid))))
+            (Tstruct _thread_info noattr)) _alloc
+          (tptr (talignas 2%N (tptr tvoid)))))
       (Sassign
         (Efield
           (Ederef
@@ -1542,8 +1639,9 @@ Definition f_garbage_collect := {|
                   (Tstruct _heap noattr)) _spaces
                 (tarray (Tstruct _space noattr) 12))
               (Econst_int (Int.repr 0) tint) (tptr (Tstruct _space noattr)))
-            (Tstruct _space noattr)) _next (tptr (tptr tvoid)))
-        (Etempvar _t'9 (tptr (tptr tvoid)))))
+            (Tstruct _space noattr)) _next
+          (tptr (talignas 2%N (tptr tvoid))))
+        (Etempvar _t'9 (tptr (talignas 2%N (tptr tvoid))))))
     (Ssequence
       (Ssequence
         (Sset _i (Econst_int (Int.repr 0) tint))
@@ -1567,8 +1665,10 @@ Definition f_garbage_collect := {|
                         (Ebinop Oadd (Etempvar _i tint)
                           (Econst_int (Int.repr 1) tint) tint)
                         (tptr (Tstruct _space noattr)))
-                      (Tstruct _space noattr)) _start (tptr (tptr tvoid))))
-                (Sifthenelse (Ebinop Oeq (Etempvar _t'6 (tptr (tptr tvoid)))
+                      (Tstruct _space noattr)) _start
+                    (tptr (talignas 2%N (tptr tvoid)))))
+                (Sifthenelse (Ebinop Oeq
+                               (Etempvar _t'6 (tptr (talignas 2%N (tptr tvoid))))
                                (Ecast (Econst_int (Int.repr 0) tint)
                                  (tptr tvoid)) tint)
                   (Ssequence
@@ -1585,7 +1685,7 @@ Definition f_garbage_collect := {|
                               (Etempvar _i tint)
                               (tptr (Tstruct _space noattr)))
                             (Tstruct _space noattr)) _limit
-                          (tptr (tptr tvoid))))
+                          (tptr (talignas 2%N (tptr tvoid)))))
                       (Ssequence
                         (Sset _t'8
                           (Efield
@@ -1599,10 +1699,12 @@ Definition f_garbage_collect := {|
                                 (Etempvar _i tint)
                                 (tptr (Tstruct _space noattr)))
                               (Tstruct _space noattr)) _start
-                            (tptr (tptr tvoid))))
+                            (tptr (talignas 2%N (tptr tvoid)))))
                         (Sset _w
-                          (Ebinop Osub (Etempvar _t'7 (tptr (tptr tvoid)))
-                            (Etempvar _t'8 (tptr (tptr tvoid))) tint))))
+                          (Ebinop Osub
+                            (Etempvar _t'7 (tptr (talignas 2%N (tptr tvoid))))
+                            (Etempvar _t'8 (tptr (talignas 2%N (tptr tvoid))))
+                            tint))))
                     (Scall None
                       (Evar _create_space (Tfunction
                                             (Tcons
@@ -1677,7 +1779,7 @@ Definition f_garbage_collect := {|
                             (Etempvar _i tint)
                             (tptr (Tstruct _space noattr)))
                           (Tstruct _space noattr)) _limit
-                        (tptr (tptr tvoid))))
+                        (tptr (talignas 2%N (tptr tvoid)))))
                     (Ssequence
                       (Sset _t'2
                         (Efield
@@ -1691,7 +1793,7 @@ Definition f_garbage_collect := {|
                               (Etempvar _i tint)
                               (tptr (Tstruct _space noattr)))
                             (Tstruct _space noattr)) _start
-                          (tptr (tptr tvoid))))
+                          (tptr (talignas 2%N (tptr tvoid)))))
                       (Ssequence
                         (Sset _t'3
                           (Efield
@@ -1706,7 +1808,7 @@ Definition f_garbage_collect := {|
                                   (Econst_int (Int.repr 1) tint) tint)
                                 (tptr (Tstruct _space noattr)))
                               (Tstruct _space noattr)) _limit
-                            (tptr (tptr tvoid))))
+                            (tptr (talignas 2%N (tptr tvoid)))))
                         (Ssequence
                           (Sset _t'4
                             (Efield
@@ -1721,15 +1823,15 @@ Definition f_garbage_collect := {|
                                     (Econst_int (Int.repr 1) tint) tint)
                                   (tptr (Tstruct _space noattr)))
                                 (Tstruct _space noattr)) _next
-                              (tptr (tptr tvoid))))
+                              (tptr (talignas 2%N (tptr tvoid)))))
                           (Sifthenelse (Ebinop Ole
                                          (Ebinop Osub
-                                           (Etempvar _t'1 (tptr (tptr tvoid)))
-                                           (Etempvar _t'2 (tptr (tptr tvoid)))
+                                           (Etempvar _t'1 (tptr (talignas 2%N (tptr tvoid))))
+                                           (Etempvar _t'2 (tptr (talignas 2%N (tptr tvoid))))
                                            tint)
                                          (Ebinop Osub
-                                           (Etempvar _t'3 (tptr (tptr tvoid)))
-                                           (Etempvar _t'4 (tptr (tptr tvoid)))
+                                           (Etempvar _t'3 (tptr (talignas 2%N (tptr tvoid))))
+                                           (Etempvar _t'4 (tptr (talignas 2%N (tptr tvoid))))
                                            tint) tint)
                             (Ssequence
                               (Scall None
@@ -1769,7 +1871,7 @@ Definition f_reset_heap := {|
   fn_params := ((_h, (tptr (Tstruct _heap noattr))) :: nil);
   fn_vars := nil;
   fn_temps := ((_i, tint) :: (_t'2, (tptr (Tstruct __IO_FILE noattr))) ::
-               (_t'1, (tptr (tptr tvoid))) :: nil);
+               (_t'1, (tptr (talignas 2%N (tptr tvoid)))) :: nil);
   fn_body :=
 (Ssequence
   (Ssequence
@@ -1799,7 +1901,7 @@ Definition f_reset_heap := {|
                       (Tstruct _heap noattr)) _spaces
                     (tarray (Tstruct _space noattr) 12)) (Etempvar _i tint)
                   (tptr (Tstruct _space noattr))) (Tstruct _space noattr))
-              _start (tptr (tptr tvoid))))
+              _start (tptr (talignas 2%N (tptr tvoid)))))
           (Sassign
             (Efield
               (Ederef
@@ -1809,7 +1911,8 @@ Definition f_reset_heap := {|
                       (Tstruct _heap noattr)) _spaces
                     (tarray (Tstruct _space noattr) 12)) (Etempvar _i tint)
                   (tptr (Tstruct _space noattr))) (Tstruct _space noattr))
-              _next (tptr (tptr tvoid))) (Etempvar _t'1 (tptr (tptr tvoid))))))
+              _next (tptr (talignas 2%N (tptr tvoid))))
+            (Etempvar _t'1 (tptr (talignas 2%N (tptr tvoid)))))))
       (Sset _i
         (Ebinop Oadd (Etempvar _i tint) (Econst_int (Int.repr 1) tint) tint)))))
 |}.
@@ -1819,7 +1922,7 @@ Definition f_free_heap := {|
   fn_callconv := cc_default;
   fn_params := ((_h, (tptr (Tstruct _heap noattr))) :: nil);
   fn_vars := nil;
-  fn_temps := ((_i, tint) :: (_p, (tptr (tptr tvoid))) ::
+  fn_temps := ((_i, tint) :: (_p, (tptr (talignas 2%N (tptr tvoid)))) ::
                (_t'1, (tptr (Tstruct __IO_FILE noattr))) :: nil);
   fn_body :=
 (Ssequence
@@ -1851,14 +1954,15 @@ Definition f_free_heap := {|
                         (Tstruct _heap noattr)) _spaces
                       (tarray (Tstruct _space noattr) 12)) (Etempvar _i tint)
                     (tptr (Tstruct _space noattr))) (Tstruct _space noattr))
-                _start (tptr (tptr tvoid))))
-            (Sifthenelse (Ebinop One (Etempvar _p (tptr (tptr tvoid)))
+                _start (tptr (talignas 2%N (tptr tvoid)))))
+            (Sifthenelse (Ebinop One
+                           (Etempvar _p (tptr (talignas 2%N (tptr tvoid))))
                            (Ecast (Econst_int (Int.repr 0) tint)
                              (tptr tvoid)) tint)
               (Scall None
                 (Evar _free (Tfunction (Tcons (tptr tvoid) Tnil) tvoid
                               cc_default))
-                ((Etempvar _p (tptr (tptr tvoid))) :: nil))
+                ((Etempvar _p (tptr (talignas 2%N (tptr tvoid)))) :: nil))
               Sskip)))
         (Sset _i
           (Ebinop Oadd (Etempvar _i tint) (Econst_int (Int.repr 1) tint)
@@ -1888,13 +1992,15 @@ Definition composites : list composite_definition :=
     (__unused2, (tarray tschar 40)) :: nil)
    noattr ::
  Composite _thread_info Struct
-   ((_alloc, (tptr (tptr tvoid))) :: (_limit, (tptr (tptr tvoid))) ::
+   ((_alloc, (tptr (talignas 2%N (tptr tvoid)))) ::
+    (_limit, (tptr (talignas 2%N (tptr tvoid)))) ::
     (_heap, (tptr (Tstruct _heap noattr))) ::
-    (_args, (tarray (tptr tvoid) 1024)) :: nil)
+    (_args, (tarray (talignas 2%N (tptr tvoid)) 1024)) :: nil)
    noattr ::
  Composite _space Struct
-   ((_start, (tptr (tptr tvoid))) :: (_next, (tptr (tptr tvoid))) ::
-    (_limit, (tptr (tptr tvoid))) :: nil)
+   ((_start, (tptr (talignas 2%N (tptr tvoid)))) ::
+    (_next, (tptr (talignas 2%N (tptr tvoid)))) ::
+    (_limit, (tptr (talignas 2%N (tptr tvoid)))) :: nil)
    noattr ::
  Composite _heap Struct
    ((_spaces, (tarray (Tstruct _space noattr) 12)) :: nil)
