theories/CertiGC/vst/proof/verif_forward.v
@@ -31,7 +31,7 @@ Qed.
 Lemma sapi_ptr_val: forall p m n,
     isptr p -> Int.min_signed <= n <= Int.max_signed ->
     (force_val
-       (sem_add_ptr_int tvalue Signed (offset_val (WORD_SIZE * m) p)
+       (sem_add_ptr_int int_or_ptr_type Signed (offset_val (WORD_SIZE * m) p)
                         (vint n))) = offset_val (WORD_SIZE * (m + n)) p.
 Proof.
   intros. rewrite sem_add_pi_ptr_special; [| easy | | easy].
@@ -43,11 +43,11 @@ Lemma sapil_ptr_val: forall p m n,
     isptr p ->
     if Archi.ptr64 then
       force_val
-        (sem_add_ptr_long tvalue (offset_val (WORD_SIZE * m) p)
+        (sem_add_ptr_long int_or_ptr_type (offset_val (WORD_SIZE * m) p)
                           (Vlong (Int64.repr n))) = offset_val (WORD_SIZE * (m + n)) p
     else
       force_val
-        (sem_add_ptr_int tvalue Signed (offset_val (WORD_SIZE * m) p)
+        (sem_add_ptr_int int_or_ptr_type Signed (offset_val (WORD_SIZE * m) p)
                          (vint n)) = offset_val (WORD_SIZE * (m + n)) p.
 Proof.
   intros. simpl.
@@ -56,12 +56,12 @@ Proof.
 Qed.
 
 Lemma data_at_mfs_eq: forall g v i sh nv,
-    field_compatible tvalue [] (offset_val (WORD_SIZE * i) nv) ->
+    field_compatible int_or_ptr_type [] (offset_val (WORD_SIZE * i) nv) ->
     0 <= i < Zlength (block_fields (heapgraph_block g v)) ->
-    data_at sh (tarray tvalue i) (sublist 0 i (heapgraph_block_cells_vals g v)) nv *
-    field_at sh tvalue [] (Znth i (heapgraph_block_cells_vals g v))
+    data_at sh (tarray int_or_ptr_type i) (sublist 0 i (heapgraph_block_cells_vals g v)) nv *
+    field_at sh int_or_ptr_type [] (Znth i (heapgraph_block_cells_vals g v))
              (offset_val (WORD_SIZE * i) nv) =
-    data_at sh (tarray tvalue (i + 1))
+    data_at sh (tarray int_or_ptr_type (i + 1))
             (sublist 0 (i + 1) (heapgraph_block_cells_vals g v)) nv.
 Proof.
   intros. rewrite field_at_data_at. unfold field_address.
@@ -69,7 +69,7 @@ Proof.
   simpl nested_field_offset. rewrite offset_offset_val.
   replace (WORD_SIZE * i + 0) with (WORD_SIZE * i)%Z by lia.
   rewrite <- (data_at_singleton_array_eq
-                sh tvalue _ [Znth i (heapgraph_block_cells_vals g v)]) by reflexivity.
+                sh int_or_ptr_type _ [Znth i (heapgraph_block_cells_vals g v)]) by reflexivity.
   rewrite <- fields_eq_length in H0.
   rewrite (data_at_tarray_value
              sh (i + 1) i nv (sublist 0 (i + 1) (heapgraph_block_cells_vals g v))
@@ -84,7 +84,7 @@ Proof.
 Qed.
 
 Lemma data_at__value_0_size: forall sh p,
-    data_at_ sh (tarray tvalue 0) p |-- emp.
+    data_at_ sh (tarray int_or_ptr_type 0) p |-- emp.
 Proof. intros. rewrite data_at__eq. apply data_at_zero_array_inv; reflexivity. Qed.
 
 Lemma data_at_minus1_address: forall sh v p,
@@ -130,9 +130,6 @@ Proof.
     assert (0 <= Znth z (live_roots_indices f_info) < MAX_ARGS) by
         (apply (fi_index_range f_info), Znth_In; assumption).
     forward; rewrite H12. 1: entailer!.
-    {
-      admit.
-    }
     assert_PROP (valid_int_or_ptr (root2val g root)). {
       gather_SEP (graph_rep _) (outlier_rep _).
       sep_apply (root_valid_int_or_ptr _ _ _ _ H13 H5). entailer!. }
@@ -201,7 +198,7 @@ Proof.
       assert (P |-- (weak_derives P (valid_pointer (Vptr b i) * TT) && emp) * P). {
         apply weak_derives_strong. subst. sep_apply (graph_rep_vertex_rep g a H19).
         Intros shh. unfold vertex_rep, vertex_at. remember (heapgraph_block_cells_vals g a).
-        sep_apply (data_at_valid_ptr shh (tarray tvalue (Zlength l)) l (heapgraph_block_ptr g a)).
+        sep_apply (data_at_valid_ptr shh (tarray int_or_ptr_type (Zlength l)) l (heapgraph_block_ptr g a)).
         - apply readable_nonidentity, writable_readable_share. assumption.
         - subst l. simpl. rewrite fields_eq_length.
           rewrite Z.max_r; pose proof (block_fields__range (heapgraph_block g a)); lia.
@@ -242,9 +239,6 @@ Proof.
              rewrite isptr_offset_val.
              apply heapgraph_generation_base__isptr, H9; assumption. }
            forward.
-           {
-             admit.
-           }
            rewrite Znth_0_cons.
            gather_SEP (data_at _ _ _ _)
                       (data_at _ _ _ _).
@@ -370,9 +364,9 @@ Proof.
                      temp _p p_addr;
                      temp _depth (vint depth))
               SEP (vertex_rep shv g a;
-                   data_at sht (tarray tvalue i)
+                   data_at sht (tarray int_or_ptr_type i)
                            (sublist 0 i (heapgraph_block_cells_vals g a)) nv;
-                   data_at_ sht (tarray tvalue (n - i))
+                   data_at_ sht (tarray int_or_ptr_type (n - i))
                             (offset_val (WORD_SIZE * i) nv); FRZL FR))%assert.
            ++ pose proof (block_fields__range2 (heapgraph_block g a)). simpl in H30.
               now rewrite <- Heqn in H30.
@@ -384,25 +378,24 @@ Proof.
            ++ unfold vertex_rep, vertex_at. Intros.
               rewrite fields_eq_length, <- Heqn. forward.
               ** entailer!. pose proof (mfv_all_is_ptr_or_int _ _ H9 H10 H19).
-                 rewrite Forall_forall in H42.
-                 admit.
-                 (* apply H42, Znth_In.
-                 rewrite fields_eq_length. assumption. *)
+                 rewrite Forall_forall in H45.
+                 apply H45, Znth_In.
+                 now rewrite fields_eq_length.
               ** rewrite (data_at__tarray_value _ _ 1) by lia. Intros.
                  rewrite data_at__singleton_array_eq.
                  assert_PROP
-                   (field_compatible tvalue []
+                   (field_compatible int_or_ptr_type []
                                      (offset_val (WORD_SIZE * i) nv)) by
                      (sep_apply (data_at__local_facts
-                                   sht tvalue
+                                   sht int_or_ptr_type
                                    (offset_val (WORD_SIZE * i) nv)); entailer!).
                  assert_PROP
                    ((if Archi.ptr64 then
-                      force_val (sem_add_ptr_long tvalue
+                      force_val (sem_add_ptr_long int_or_ptr_type
                                                   nv (Vlong (Int64.repr i)))
-                     else force_val (sem_add_ptr_int tvalue
+                     else force_val (sem_add_ptr_int int_or_ptr_type
                                                      Signed nv (vint i)))=
-                    field_address tvalue []
+                    field_address int_or_ptr_type []
                                   (offset_val (WORD_SIZE * i) nv)). {
                    unfold field_address. rewrite if_true by assumption.
                    clear. entailer!. } simpl in H32.
@@ -476,17 +469,17 @@ Proof.
                 subst l'. rewrite fields_eq_length.
                 apply (proj1 (block_fields__range (heapgraph_block g' a))). }
               rewrite data_at_tarray_value_split_1 by assumption. Intros.
-              assert_PROP (force_val (sem_add_ptr_int tvalue Signed
+              assert_PROP (force_val (sem_add_ptr_int int_or_ptr_type Signed
                                                       (heapgraph_block_ptr g' a) (vint 0)) =
-                           field_address tvalue [] (heapgraph_block_ptr g' a)). {
+                           field_address int_or_ptr_type [] (heapgraph_block_ptr g' a)). {
                 clear. entailer!. unfold field_address. rewrite if_true by assumption.
                 simpl. rewrite isptr_offset_val_zero. 1: reflexivity.
-                destruct H7 ; try assumption ; admit. } forward. clear H38.
+                destruct H7 ; try assumption. } forward. clear H38.
               sep_apply (field_at_data_at_cancel
-                           sh' tvalue nv (heapgraph_block_ptr g' a)).
+                           sh' int_or_ptr_type nv (heapgraph_block_ptr g' a)).
               gather_SEP
                 (data_at _ (if Archi.ptr64 then tulong else tuint) _ _)
-                (data_at _ tvalue nv _)
+                (data_at _ int_or_ptr_type nv _)
                 (data_at _ _ _ _).
               rewrite H30. subst l'.
               rewrite <- lmc_vertex_rep_eq.
@@ -565,7 +558,7 @@ Proof.
                          constructor. unfold thread_info_relation. entailer!.
                  --- change (Tpointer tvoid {| attr_volatile := false;
                                                attr_alignas := Some 2%N |})
-                       with (tvalue). Intros.
+                       with (int_or_ptr_type). Intros.
                      assert (heapgraph_has_gen g' to) by
                          (rewrite Heqg', <- lcv_graph_has_gen; assumption).
                      assert (heapgraph_has_block g' (new_copied_v g to)) by
@@ -647,7 +640,7 @@ Proof.
     localize [vertex_rep (heapgraph_generation_sh g (addr_gen v)) g v].
     unfold vertex_rep, vertex_at. Intros.
     assert_PROP (offset_val (WORD_SIZE * n) (heapgraph_block_ptr g v) =
-                 field_address (tarray tvalue
+                 field_address (tarray int_or_ptr_type
                                        (Zlength (heapgraph_block_cells_vals g v)))
                                [ArraySubsc n] (heapgraph_block_ptr g v)). {
       entailer!. unfold field_address. rewrite if_true; [simpl; f_equal|].
@@ -662,10 +655,6 @@ Proof.
     gather_SEP (data_at _ _ _ _) (data_at _ _ _ _).
     replace_SEP 0 (vertex_rep (heapgraph_generation_sh g (addr_gen v)) g v).
     1: unfold vertex_rep, vertex_at; entailer!.
-    {
-      entailer!.
-      admit.
-    }
     unlocalize [graph_rep g]. 1: apply graph_vertex_ramif_stable; assumption. thaw FR.
     unfold heapgraph_block_cells_vals.
     rewrite H12, Znth_map; [|rewrite heapgraph_block_cells_eq_length; assumption].
@@ -801,7 +790,7 @@ Proof.
         sep_apply (graph_rep_vertex_rep g v' H19).
         Intros shh. unfold vertex_rep, vertex_at. rewrite Heqv0.
         sep_apply (data_at_valid_ptr
-                     shh (tarray tvalue (Zlength (heapgraph_block_cells_vals g v')))
+                     shh (tarray int_or_ptr_type (Zlength (heapgraph_block_cells_vals g v')))
                      (heapgraph_block_cells_vals g v') (Vptr b i)).
         - apply readable_nonidentity, writable_readable_share; assumption.
         - simpl. rewrite fields_eq_length.
@@ -850,10 +839,6 @@ Proof.
             apply heapgraph_generation_base__isptr, H9; assumption.
           }
           forward.
-          {
-            entailer!.
-            admit.
-          }
           rewrite Znth_0_cons.
           gather_SEP (data_at _ _ _ _) (data_at _ _ _ _).
           replace_SEP 0 (vertex_rep (heapgraph_generation_sh g (addr_gen v')) g v').
@@ -868,7 +853,7 @@ Proof.
           forward.
           sep_apply (field_at_data_at_cancel
                        (heapgraph_generation_sh g (addr_gen v))
-                       (tarray tvalue (Zlength (heapgraph_block_cells_vals g v)))
+                       (tarray int_or_ptr_type (Zlength (heapgraph_block_cells_vals g v)))
                        (upd_Znth n (heapgraph_block_cells_vals g v)
                        (heapgraph_block_ptr g (block_copied_vertex (heapgraph_block g v'))))
                        (heapgraph_block_ptr g v)).
@@ -898,14 +883,11 @@ Proof.
           pose proof (lgd_no_dangling_dst_copied_vert g e (dst g e) H9 H19 H22 H10).
           split; [|split; [|split; [|split]]]; try reflexivity.
           ++ constructor ; try easy.
-             intuition.
-             { admit. }
-             { admit. }
+             admit. (* more coercion problems? *)
           ++ simpl forward_p2forward_t.
              rewrite H12, Heqc. simpl. now constructor.
           ++ constructor ; try easy.
-             intuition.
-             admit.
+             admit. (* more coercion problems? *)
           ++ easy.
         -- (* not yet forwarded *)
            forward. thaw FR.  freeze [0; 1; 2; 3; 4; 5] FR.
@@ -1006,9 +988,9 @@ Proof.
                      temp _p (offset_val (WORD_SIZE * n) (heapgraph_block_ptr g v));
                      temp _depth (vint depth))
               SEP (vertex_rep shv g v';
-                   data_at sht (tarray tvalue i)
+                   data_at sht (tarray int_or_ptr_type i)
                            (sublist 0 i (heapgraph_block_cells_vals g v')) nv;
-                   data_at_ sht (tarray tvalue (n' - i))
+                   data_at_ sht (tarray int_or_ptr_type (n' - i))
                             (offset_val (WORD_SIZE * i) nv); FRZL FR))%assert.
            ++ pose proof (block_fields__range2 (heapgraph_block g v')). simpl in H31.
               now rewrite <- Heqn' in H31.
@@ -1018,26 +1000,25 @@ Proof.
               rewrite data_at_zero_array_eq; [entailer! | easy..].
            ++ unfold vertex_rep, vertex_at. Intros.
               rewrite fields_eq_length, <- Heqn'. forward.
-              ** entailer!. pose proof (mfv_all_is_ptr_or_int _ _ H9 H10 H19).
-                 rewrite Forall_forall in H44.
-                 admit.
-                 (* apply H44, Znth_In. *)
-                 (* rewrite fields_eq_length. assumption. *)
+              ** entailer!. pose proof (mfv_all_is_ptr_or_int _ _ H9 H10 H19) as HH.
+                 rewrite Forall_forall in HH.
+                 apply HH, Znth_In.
+                 now rewrite fields_eq_length.
               ** rewrite (data_at__tarray_value _ _ 1) by lia. Intros.
                  rewrite data_at__singleton_array_eq.
                  assert_PROP
-                   (field_compatible tvalue []
+                   (field_compatible int_or_ptr_type []
                                      (offset_val (WORD_SIZE * i) nv)) by
                      (sep_apply (data_at__local_facts
-                                   sht tvalue
+                                   sht int_or_ptr_type
                                    (offset_val (WORD_SIZE * i) nv)); entailer!).
                  assert_PROP
                    ((if Archi.ptr64 then
-                      force_val (sem_add_ptr_long tvalue
+                      force_val (sem_add_ptr_long int_or_ptr_type
                                                   nv (Vlong (Int64.repr i)))
-                     else force_val (sem_add_ptr_int tvalue
+                     else force_val (sem_add_ptr_int int_or_ptr_type
                                                      Signed nv (vint i))) =
-                    field_address tvalue []
+                    field_address int_or_ptr_type []
                                   (offset_val (WORD_SIZE * i) nv)). {
                    unfold field_address. rewrite if_true by assumption.
                    clear. entailer!. } simpl in H33.
@@ -1108,20 +1089,20 @@ Proof.
                 subst l'. rewrite fields_eq_length.
                 apply (proj1 (block_fields__range (heapgraph_block g' v'))). }
               rewrite data_at_tarray_value_split_1 by assumption. Intros.
-              assert_PROP (force_val (sem_add_ptr_int tvalue Signed
+              assert_PROP (force_val (sem_add_ptr_int int_or_ptr_type Signed
                                                       (heapgraph_block_ptr g' v') (vint 0))
                            =
-                           field_address tvalue [] (heapgraph_block_ptr g' v')).
+                           field_address int_or_ptr_type [] (heapgraph_block_ptr g' v')).
               {
                 clear. entailer!. unfold field_address. rewrite if_true by assumption.
                 simpl. rewrite isptr_offset_val_zero. 1: reflexivity.
-                destruct H7 ; try assumption ; admit.
+                now destruct H7.
               }
               forward. clear H39.
               sep_apply (field_at_data_at_cancel
-                           sh' tvalue nv (heapgraph_block_ptr g' v')).
+                           sh' int_or_ptr_type nv (heapgraph_block_ptr g' v')).
               gather_SEP (data_at sh' (if Archi.ptr64 then tulong else tuint) _ _)
-                         (data_at sh' tvalue _ _) (data_at _ _ _ _).
+                         (data_at sh' int_or_ptr_type _ _) (data_at _ _ _ _).
               rewrite H31. subst l'.
               rewrite <- lmc_vertex_rep_eq.
               thaw FR1.
@@ -1181,7 +1162,7 @@ Proof.
               rewrite H31.
               sep_apply (field_at_data_at_cancel
                            shh
-                           (tarray tvalue (Zlength (heapgraph_block_cells_vals g' v)))
+                           (tarray int_or_ptr_type (Zlength (heapgraph_block_cells_vals g' v)))
                            (upd_Znth n (heapgraph_block_cells_vals g' v) (heapgraph_block_ptr g' a))
                            (heapgraph_block_ptr g' v)).
               gather_SEP (data_at shh _ _ _) (data_at shh _ _ _).
